Add some more info to ids_unique to make the final conneciton theorem easier to prove

icing/CakeMLtoFloVerLemsScript.sml
@@ -11,133 +11,133 @@ open preamble;
 val _ = new_theory "CakeMLtoFloVerLems";
 
 Definition freevars_def:
-  freevars [] = EMPTY ∧
-  freevars [ast$Var n] = { n } ∧
-  freevars [Lit l] = EMPTY ∧
-  freevars [Raise e] = freevars [e] ∧
+  freevars [] = EMPTY /\
+  freevars [ast$Var n] = { n } /\
+  freevars [Lit l] = EMPTY /\
+  freevars [Raise e] = freevars [e] /\
   freevars [Handle e pes] =
-    FOLDL (λ vars. λ (p,e). (freevars [e]) ∪ vars) (freevars [e]) pes ∧
-  freevars [Con id es] = freevars es ∧
-  freevars [Fun s e] = freevars [e] DIFF { Short s } ∧
-  freevars [App op es] = freevars es ∧
-  freevars [Log lop e1 e2] = (freevars [e1] ∪ freevars [e2]) ∧
-  freevars [If e1 e2 e3] = (freevars [e1] ∪ freevars [e2] ∪ freevars [e3]) ∧
+    FOLDL (\ vars. \ (p,e). (freevars [e]) UNION vars) (freevars [e]) pes /\
+  freevars [Con id es] = freevars es /\
+  freevars [Fun s e] = freevars [e] DIFF { Short s } /\
+  freevars [App op es] = freevars es /\
+  freevars [Log lop e1 e2] = (freevars [e1] UNION freevars [e2]) /\
+  freevars [If e1 e2 e3] = (freevars [e1] UNION freevars [e2] UNION freevars [e3]) /\
   freevars [Mat e pes] =
-    FOLDL (λ vars. λ (p,e). (freevars [e]) ∪ vars) (freevars [e]) pes ∧
+    FOLDL (\ vars. \ (p,e). (freevars [e]) UNION vars) (freevars [e]) pes /\
   freevars [Let x e1 e2] =
-    freevars [e1] ∪
-    (freevars [e2] DIFF (case x of | NONE => EMPTY | SOME s => { Short s })) ∧
-  freevars [Letrec fs e] = EMPTY (* TODO *) ∧
-  freevars [Tannot e t] = freevars [e] ∧
-  freevars [Lannot e l] = freevars [e] ∧
-  freevars [FpOptimise opt e] = freevars [e] ∧
+    freevars [e1] UNION
+    (freevars [e2] DIFF (case x of | NONE => EMPTY | SOME s => { Short s })) /\
+  freevars [Letrec fs e] = EMPTY (* TODO *) /\
+  freevars [Tannot e t] = freevars [e] /\
+  freevars [Lannot e l] = freevars [e] /\
+  freevars [FpOptimise opt e] = freevars [e] /\
   freevars (e1::es) =
-    freevars [e1] ∪ freevars es
+    freevars [e1] UNION freevars es
 Termination
-  wf_rel_tac ‘measure exp6_size’ \\ fs[]
-  \\ Induct_on ‘pes’ \\ fs[]
+  wf_rel_tac `measure exp6_size` \\ fs[]
+  \\ Induct_on `pes` \\ fs[]
   \\ rpt strip_tac \\ simp[astTheory.exp_size_def]  \\ rveq
   \\ res_tac
   >- (simp[astTheory.exp_size_def])
-  \\ first_x_assum (qspec_then ‘e’ assume_tac) \\ fs[]
+  \\ first_x_assum (qspec_then `e` assume_tac) \\ fs[]
 End
 
 Theorem lookupCMLVar_id_l:
-  lookupCMLVar x ids = SOME (y, n) ⇒
+  lookupCMLVar x ids = SOME (y, n) ==>
   x = y
 Proof
-  Induct_on ‘ids’ \\ fs[lookupCMLVar_def, updateTheory.FIND_def]
-  \\ strip_tac \\ rename1 ‘(λ (m,i). x = m) h’ \\ Cases_on ‘h’ \\  fs[]
+  Induct_on `ids` \\ fs[lookupCMLVar_def, updateTheory.FIND_def]
+  \\ strip_tac \\ rename1 `(\ (m,i). x = m) h` \\ Cases_on `h` \\  fs[]
   \\ TOP_CASE_TAC \\ fs[]
 QED
 
 Theorem lookupFloVerVar_id_r:
-  lookupFloVerVar n ids = SOME (x,m) ⇒
+  lookupFloVerVar n ids = SOME (x,m) ==>
   n = m
 Proof
-  Induct_on ‘ids’ \\ fs[lookupFloVerVar_def, updateTheory.FIND_def]
-  \\ strip_tac \\ rename1 ‘(λ (m,i). n = i) h’ \\ Cases_on ‘h’ \\  fs[]
+  Induct_on `ids` \\ fs[lookupFloVerVar_def, updateTheory.FIND_def]
+  \\ strip_tac \\ rename1 `(\ (m,i). n = i) h` \\ Cases_on `h` \\  fs[]
   \\ TOP_CASE_TAC \\ fs[]
 QED
 
 Theorem toFloVerExp_App_cases:
-  ∀ varMap freshId op exps theIds1 freshId1 fexp.
-    toFloVerExp varMap freshId (App op exps) = SOME (theIds1, freshId1, fexp) ⇒
-    (∃ w.
-     op = FpFromWord ∧ exps = [Lit (Word64 w)] ∧
-     fexp = Expressions$Const M64 w ∧
-     varMap = theIds1 ∧ freshId = freshId1) ∨
-    (∃ e fexp2.
-       (op = FP_uop FP_Neg ∧ exps = [e] ∧
-       toFloVerExp varMap freshId e = SOME (theIds1, freshId1, fexp2) ∧
-       fexp = Unop Neg fexp2)) ∨
-    (∃ e1 e2 bop theIds2 freshId2 fexp1 fexp2.
-      (op = FP_bop bop ∧ exps = [e1; e2] ∧
-       toFloVerExp varMap freshId e1 = SOME (theIds2, freshId2, fexp1) ∧
-       toFloVerExp theIds2 freshId2 e2 = SOME (theIds1, freshId1, fexp2) ∧
-       fexp = Binop (fpBopToFloVer bop) fexp1 fexp2)) ∨
-    (∃ e1 e2 e3 theIds2 theIds3 freshId2 freshId3 fexp1 fexp2 fexp3.
-      (op = FP_top FP_Fma ∧ exps = [e1; e2; e3] ∧
-       toFloVerExp varMap freshId e1 = SOME (theIds2, freshId2, fexp1) ∧
-       toFloVerExp theIds2 freshId2 e2 = SOME (theIds3, freshId3, fexp2) ∧
-       toFloVerExp theIds3 freshId3 e3 = SOME (theIds1, freshId1, fexp3) ∧
+  ! varMap freshId op exps theIds1 freshId1 fexp.
+    toFloVerExp varMap freshId (App op exps) = SOME (theIds1, freshId1, fexp) ==>
+    (? w.
+     op = FpFromWord /\ exps = [Lit (Word64 w)] /\
+     fexp = Expressions$Const M64 w /\
+     varMap = theIds1 /\ freshId = freshId1) \/
+    (? e fexp2.
+       (op = FP_uop FP_Neg /\ exps = [e] /\
+       toFloVerExp varMap freshId e = SOME (theIds1, freshId1, fexp2) /\
+       fexp = Unop Neg fexp2)) \/
+    (? e1 e2 bop theIds2 freshId2 fexp1 fexp2.
+      (op = FP_bop bop /\ exps = [e1; e2] /\
+       toFloVerExp varMap freshId e1 = SOME (theIds2, freshId2, fexp1) /\
+       toFloVerExp theIds2 freshId2 e2 = SOME (theIds1, freshId1, fexp2) /\
+       fexp = Binop (fpBopToFloVer bop) fexp1 fexp2)) \/
+    (? e1 e2 e3 theIds2 theIds3 freshId2 freshId3 fexp1 fexp2 fexp3.
+      (op = FP_top FP_Fma /\ exps = [e1; e2; e3] /\
+       toFloVerExp varMap freshId e1 = SOME (theIds2, freshId2, fexp1) /\
+       toFloVerExp theIds2 freshId2 e2 = SOME (theIds3, freshId3, fexp2) /\
+       toFloVerExp theIds3 freshId3 e3 = SOME (theIds1, freshId1, fexp3) /\
        fexp = Fma fexp2 fexp3 fexp1))
 Proof
   fs[toFloVerExp_def, option_case_eq, list_case_eq]
-  \\ Cases_on ‘op’ \\ fs[]
-  \\ TRY (Cases_on ‘f’)
+  \\ Cases_on `op` \\ fs[]
+  \\ TRY (Cases_on `f`)
   \\ fs[list_case_eq, option_case_eq, pair_case_eq]
   \\ rpt strip_tac \\ fs[] \\ rveq \\ fs[]
-  \\ Cases_on ‘e1’ \\ TRY (Cases_on ‘l’) \\ fs[toFloVerConst_def]
+  \\ Cases_on `e1` \\ TRY (Cases_on `l`) \\ fs[toFloVerConst_def]
 QED
 
 Theorem toFloVerExp_usedVars:
-  ∀ ids freshId e ids2 freshId2 fexp.
-    toFloVerExp ids freshId e = SOME (ids2, freshId2, fexp) ⇒
-    ∀ n. freshId ≤ n ∧ n < freshId2 ⇒
+  ! ids freshId e ids2 freshId2 fexp.
+    toFloVerExp ids freshId e = SOME (ids2, freshId2, fexp) ==>
+    ! n. freshId <= n /\ n < freshId2 ==>
       n IN domain (usedVars (fexp))
 Proof
   ho_match_mp_tac toFloVerExp_ind
   \\ rpt strip_tac \\ TRY (fs[toFloVerExp_def] \\ NO_TAC)
   >- (
-   qpat_x_assum ‘_ = SOME _’ mp_tac \\ fs[toFloVerExp_def]
+   qpat_x_assum `_ = SOME _` mp_tac \\ fs[toFloVerExp_def]
    \\ rpt (TOP_CASE_TAC \\ fs[])
    \\ rpt strip_tac \\ rveq \\ fs[usedVars_def])
   \\ first_x_assum (mp_then Any assume_tac toFloVerExp_App_cases)
   \\ fs[] \\ rveq \\ fs[]
   \\ simp[Once usedVars_def, domain_union]
   \\ TRY (metis_tac[])
-  \\ TRY (Cases_on ‘n < freshId2'’\\ fs[] \\ metis_tac[])
-  \\ TRY (Cases_on ‘n < freshId2'’\\ fs[] \\ TRY (metis_tac[])
-          \\ Cases_on ‘n < freshId3’ \\ fs[] \\ metis_tac[])
+  \\ TRY (Cases_on `n < freshId2'`\\ fs[] \\ metis_tac[])
+  \\ TRY (Cases_on `n < freshId2'`\\ fs[] \\ TRY (metis_tac[])
+          \\ Cases_on `n < freshId3` \\ fs[] \\ metis_tac[])
 QED
 
 Theorem getInterval_inv:
-  getInterval e = SOME (x,lo,hi) ⇒
-  freevars [e] = { Short x } ∧
-  ∃ w1 w2.
+  getInterval e = SOME (x,lo,hi) ==>
+  freevars [e] = { Short x } /\
+  ? w1 w2.
   e = Log And (App (FP_cmp FP_LessEqual) [Lit (Word64 w1); Var (Short x)])
-  (App (FP_cmp FP_LessEqual) [Var (Short x); Lit (Word64 w2)]) ∧
-  lo = fp64_to_real w1 ∧
-  hi = fp64_to_real w2 ∧
-  fp64_isFinite w1 ∧
+  (App (FP_cmp FP_LessEqual) [Var (Short x); Lit (Word64 w2)]) /\
+  lo = fp64_to_real w1 /\
+  hi = fp64_to_real w2 /\
+  fp64_isFinite w1 /\
   fp64_isFinite w2
 Proof
-  Cases_on ‘e’ \\ simp[getInterval_def]
+  Cases_on `e` \\ simp[getInterval_def]
   \\ rpt (TOP_CASE_TAC \\ fs[])
   \\ rpt strip_tac \\ rveq \\ fs[freevars_def]
 QED
 
 Theorem toFloVerPre_freevar_FIND:
-  ∀ cake_P ids floverP dVars.
-  toFloVerPre cake_P ids = SOME (floverP, dVars) ⇒
-  ∀ x. x IN freevars cake_P ⇒
-  ∃ n m. lookupCMLVar x ids = SOME (x, n) ∧
-  FIND (λ m. n = m) dVars = SOME m
+  ! cake_P ids floverP dVars.
+  toFloVerPre cake_P ids = SOME (floverP, dVars) ==>
+  ! x. x IN freevars cake_P ==>
+  ? n m. lookupCMLVar x ids = SOME (x, n) /\
+  FIND (\ m. n = m) dVars = SOME m
 Proof
   ho_match_mp_tac toFloVerPre_ind
   \\ rpt strip_tac \\ fs[toFloVerPre_def]
-  \\ qpat_x_assum ‘_ = SOME (_, _)’ mp_tac
+  \\ qpat_x_assum `_ = SOME (_, _)` mp_tac
   \\ reverse TOP_CASE_TAC \\ fs[]
   >- (
     rpt (TOP_CASE_TAC \\ fs[])
@@ -161,35 +161,40 @@ QED
 
 Definition ids_unique_def:
   ids_unique ids (freshId:num) =
-  ((∀ x y z.
-    lookupCMLVar x ids = SOME (x, y) ∧
-    lookupFloVerVar z ids = SOME (x, z) ⇒
-    z = y) ∧
-  (∀ x y z.
-    lookupCMLVar (Short x) ids = SOME (Short x, z) ∧
-    lookupFloVerVar z ids = SOME (Short y, z) ⇒
-    x = y) ∧
-  (∀ x y z.
-    lookupCMLVar x ids = SOME (x,z) ∧
-    lookupCMLVar y ids = SOME (y,z) ⇒
-    x = y) ∧
-  (∀ x y z.
-    lookupFloVerVar x ids = SOME (z,x) ∧
-    lookupFloVerVar y ids = SOME (z,y) ⇒
-    x = y) ∧
+  ((! x y z.
+    lookupCMLVar x ids = SOME (x, y) /\
+    lookupFloVerVar z ids = SOME (x, z) ==>
+    z = y) /\
+  (! x y z.
+    lookupCMLVar (Short x) ids = SOME (Short x, z) /\
+    lookupFloVerVar z ids = SOME (Short y, z) ==>
+    x = y) /\
+  (! x y z.
+    lookupCMLVar x ids = SOME (x,z) /\
+    lookupCMLVar y ids = SOME (y,z) ==>
+    x = y) /\
+  (! x y z.
+    lookupFloVerVar x ids = SOME (z,x) /\
+    lookupFloVerVar y ids = SOME (z,y) ==>
+    x = y) /\
+  (! x y.
+    lookupFloVerVar x ids = SOME (y, x) ==>
+    lookupCMLVar y ids = SOME (y,x)) /\
+  (! x y.
+    lookupCMLVar y ids = SOME (y,x) ==>
+    lookupFloVerVar x ids = SOME (y, x)) /\
   (∀ x y.
-    lookupFloVerVar x ids = SOME (y, x) ⇒
-    lookupCMLVar y ids = SOME (y,x)) ∧
-  (∀ x y.
-    lookupCMLVar y ids = SOME (y,x) ⇒
-    lookupFloVerVar x ids = SOME (y, x)) ∧
-  (∀ id. freshId ≤ id ⇒ lookupFloVerVar id ids = NONE) ∧
-  (∀ x y. lookupCMLVar x ids = SOME (x, y) ⇒
-     y < freshId))
+    MEM (x,y) ids ⇒
+    lookupFloVerVar y ids = SOME (x,y) ∧
+    lookupCMLVar x ids = SOME (x,y)) ∧
+  (! id. freshId <= id ==> lookupFloVerVar id ids = NONE) /\
+  (! x y. lookupCMLVar x ids = SOME (x, y) ==>
+   y < freshId) /\
+  ALL_DISTINCT ids)
 End
 
 Theorem lookupCMLVar_appendCMLVar:
-  ∀ x y freshId varMap.
+  ! x y freshId varMap.
     lookupCMLVar x (appendCMLVar y freshId varMap) =
     case lookupCMLVar y varMap of
     | NONE => lookupCMLVar x ((y,freshId)::varMap)
@@ -200,7 +205,7 @@ Proof
 QED
 
 Theorem lookupFloVerVar_appendCMLVar:
-  ∀ x y freshId varMap.
+  ! x y freshId varMap.
     lookupFloVerVar x (appendCMLVar y freshId varMap) =
     case lookupCMLVar y varMap of
     | NONE => lookupFloVerVar x ((y, freshId)::varMap)
@@ -210,52 +215,124 @@ Proof
   \\ TOP_CASE_TAC \\ fs[lookupFloVerVar_def, updateTheory.FIND_def]
 QED
 
+Theorem lookupCMLVar_not_mem:
+  ! x ids.
+  lookupCMLVar x ids = NONE ==>
+  ! y. ~ MEM (x,y) ids
+Proof
+  Induct_on `ids` \\ fs[lookupCMLVar_def]
+  \\ rpt strip_tac \\ rveq \\ fs[updateTheory.FIND_def]
+  \\ Cases_on `h` \\ fs[]
+  \\ every_case_tac \\ fs[]
+  \\ res_tac
+QED
+
+Theorem lookupCMLVar_mem:
+  ! x y ids.
+  lookupCMLVar x ids = SOME (x,y) ==>
+  MEM (x,y) ids
+Proof
+  Induct_on `ids` \\ fs[lookupCMLVar_def]
+  \\ rpt strip_tac \\ rveq \\ fs[updateTheory.FIND_def]
+  \\ Cases_on `h` \\ fs[]
+  \\ every_case_tac \\ fs[]
+  \\ res_tac
+QED
+
+Theorem lookupFloVerVar_not_mem:
+  ! y ids.
+  lookupFloVerVar y ids = NONE ==>
+  ! x. ~ MEM (x,y) ids
+Proof
+  Induct_on `ids` \\ fs[lookupFloVerVar_def]
+  \\ rpt strip_tac \\ rveq \\ fs[updateTheory.FIND_def]
+  \\ Cases_on `h` \\ fs[]
+  \\ every_case_tac \\ fs[]
+  \\ res_tac
+QED
+
+Theorem lookupFloVerVar_mem:
+  ! x y ids.
+  lookupFloVerVar x ids = SOME (y, x) ==>
+  MEM (y, x) ids
+Proof
+  Induct_on `ids` \\ fs[lookupFloVerVar_def]
+  \\ rpt strip_tac \\ rveq \\ fs[updateTheory.FIND_def]
+  \\ Cases_on `h` \\ fs[]
+  \\ every_case_tac \\ fs[]
+  \\ res_tac
+QED
+
+val tac =
+  fs[lookupFloVerVar_appendCMLVar, lookupCMLVar_appendCMLVar] \\ rfs[]
+  \\ fs[lookupFloVerVar_def, lookupCMLVar_def]
+  \\ ntac 2 (pop_assum mp_tac)
+  \\ simp[updateTheory.FIND_def]
+  \\ rpt (TOP_CASE_TAC \\ strip_tac \\ fs[] \\ rveq)
+  \\ rpt strip_tac \\ res_tac \\ rveq \\ fs[]
+  \\ fs[appendCMLVar_def] \\ TOP_CASE_TAC \\ fs[];
+
 Theorem prepareVars_is_unique:
-  ∀ ids floverVars varMap freshId.
-    prepareVars ids = SOME (floverVars, varMap, freshId) ⇒
+  ! ids floverVars varMap freshId.
+    prepareVars ids = SOME (floverVars, varMap, freshId) ==>
     ids_unique varMap freshId
 Proof
-  Induct_on ‘ids’ \\ fs[prepareVars_def]
+  Induct_on `ids` \\ fs[prepareVars_def]
   >- (
     rpt strip_tac \\ fs[] \\ rveq
     \\ fs[ids_unique_def, lookupCMLVar_def, lookupFloVerVar_def,
           updateTheory.FIND_def])
   \\ fs[option_case_eq, pair_case_eq, ids_unique_def]
   \\ rpt strip_tac \\ rveq
-  \\ fs[lookupFloVerVar_appendCMLVar, lookupCMLVar_appendCMLVar] \\ rfs[]
-  \\ fs[lookupFloVerVar_def, lookupCMLVar_def]
-  \\ ntac 2 (pop_assum mp_tac)
-  \\ simp[updateTheory.FIND_def]
-  \\ rpt (TOP_CASE_TAC \\ strip_tac \\ fs[] \\ rveq)
-  \\ rpt strip_tac \\ res_tac \\ rveq \\ fs[]
+  >- (tac)
+  >- (tac)
+  >- (tac)
+  >- (tac)
+  >- (tac)
+  >- (tac)
+  >- (
+    fs[lookupFloVerVar_appendCMLVar, appendCMLVar_def] \\ rfs[]
+    \\ rveq \\ simp[lookupFloVerVar_def, updateTheory.FIND_def]
+    \\ TOP_CASE_TAC \\ rveq \\ fs[]
+    >- (res_tac \\ fs[] \\ res_tac \\ fs[])
+    \\ res_tac \\ fs[lookupFloVerVar_def])
+  >- (
+    fs[lookupFloVerVar_appendCMLVar, appendCMLVar_def] \\ rfs[]
+    \\ rveq \\ simp[lookupCMLVar_def, updateTheory.FIND_def]
+    \\ TOP_CASE_TAC \\ rveq \\ fs[]
+    >- (res_tac \\ fs[] \\ res_tac \\ fs[])
+    \\ res_tac \\ fs[lookupCMLVar_def])
+  >- (tac)
+  >- (tac)
+  \\ imp_res_tac lookupCMLVar_not_mem \\ fs[appendCMLVar_def]
 QED
 
 Theorem prepareVars_agrees_CakeML:
-  ∀ ids floverVars varMap freshId.
-  prepareVars ids = SOME (floverVars, varMap, freshId) ⇒
-  ∀ s. MEM s ids ⇒
-  ∃ x. lookupCMLVar (Short s) varMap = SOME (Short s, x) ∧
+  ! ids floverVars varMap freshId.
+  prepareVars ids = SOME (floverVars, varMap, freshId) ==>
+  ! s. MEM s ids ==>
+  ? x. lookupCMLVar (Short s) varMap = SOME (Short s, x) /\
   MEM x floverVars
 Proof
-  Induct_on ‘ids’ \\ fs[prepareVars_def]
+  Induct_on `ids` \\ fs[prepareVars_def]
   \\ rpt strip_tac \\ rveq
   \\ fs[option_case_eq, pair_case_eq] \\ rveq
   \\ fs [lookupCMLVar_appendCMLVar, lookupCMLVar_def, updateTheory.FIND_def]
   \\ res_tac
   \\ imp_res_tac prepareVars_is_unique
-  \\ ‘s ≠ h’
+  \\ `s <> h`
      by (CCONTR_TAC \\ fs[] \\ rveq \\ fs[ids_unique_def] \\ res_tac)
   \\ fs[]
 QED
 
 Theorem prepareVars_agrees_FloVer:
-  ∀ ids floverVars varMap freshId.
-  prepareVars ids = SOME (floverVars, varMap, freshId) ⇒
-  ∀ x s. lookupFloVerVar x varMap = SOME (s, x) ⇒
-  ∃ n. s = Short n ∧ MEM n ids ∧
+  ! ids floverVars varMap freshId.
+  prepareVars ids = SOME (floverVars, varMap, freshId) ==>
+  ! x s. lookupFloVerVar x varMap = SOME (s, x) ==>
+  ? n. s = Short n /\ MEM n ids /\
   MEM x floverVars
 Proof
-  Induct_on ‘ids’
+  Induct_on `ids`
   >- (fs[prepareVars_def, lookupFloVerVar_def, updateTheory.FIND_def])
   \\ fs[prepareVars_def, option_case_eq, pair_case_eq]
   \\ rpt strip_tac \\ rveq
@@ -268,8 +345,8 @@ Proof
 QED
 
 Theorem toFloVerExp_noDowncast:
-  ∀ varMap freshId e theIds freshId2 theExp.
-    toFloVerExp varMap freshId e = SOME (theIds, freshId2, theExp) ⇒
+  ! varMap freshId e theIds freshId2 theExp.
+    toFloVerExp varMap freshId e = SOME (theIds, freshId2, theExp) ==>
     noDowncast (toRExp theExp)
 Proof
   ho_match_mp_tac toFloVerExp_ind
@@ -280,8 +357,8 @@ Proof
 QED
 
 Theorem toFloVerCmd_noDowncastFun:
-  ∀ varMap freshId f theIds freshId2 theCmd.
-    toFloVerCmd varMap freshId f = SOME (theIds, freshId2, theCmd) ⇒
+  ! varMap freshId f theIds freshId2 theCmd.
+    toFloVerCmd varMap freshId f = SOME (theIds, freshId2, theCmd) ==>
     noDowncastFun (toRCmd theCmd)
 Proof
   ho_match_mp_tac toFloVerCmd_ind
@@ -292,9 +369,9 @@ Proof
 QED
 
 Theorem is64BitEnv_prepareGamma:
-  ∀ floverVars. is64BitEnv (prepareGamma floverVars)
+  ! floverVars. is64BitEnv (prepareGamma floverVars)
 Proof
-  Induct_on ‘floverVars’ \\ fs[is64BitEnv_def, prepareGamma_def]
+  Induct_on `floverVars` \\ fs[is64BitEnv_def, prepareGamma_def]
   >- (
    rpt strip_tac
    \\ fs[FloverMapTheory.FloverMapTree_find_def,
@@ -304,8 +381,8 @@ Proof
 QED
 
 Theorem toFloVerExp_is64BitEval:
-  ∀ varMap freshId e theIds freshId2 theExp.
-    toFloVerExp varMap freshId e = SOME (theIds, freshId2, theExp) ⇒
+  ! varMap freshId e theIds freshId2 theExp.
+    toFloVerExp varMap freshId e = SOME (theIds, freshId2, theExp) ==>
     is64BitEval (toRExp theExp)
 Proof
   ho_match_mp_tac toFloVerExp_ind
@@ -316,8 +393,8 @@ Proof
 QED
 
 Theorem toFloVerCmd_is64BitBstep:
-  ∀ varMap freshId f theIds freshId2 theCmd.
-    toFloVerCmd varMap freshId f = SOME (theIds, freshId2, theCmd) ⇒
+  ! varMap freshId f theIds freshId2 theCmd.
+    toFloVerCmd varMap freshId f = SOME (theIds, freshId2, theCmd) ==>
     is64BitBstep (toRCmd theCmd)
 Proof
   ho_match_mp_tac toFloVerCmd_ind
@@ -328,36 +405,38 @@ Proof
 QED
 
 Theorem ids_unique_append:
-  ∀ x varMap freshId.
-    ids_unique varMap freshId ⇒
+  ! x varMap freshId.
+    ids_unique varMap freshId ==>
     ids_unique (appendCMLVar x freshId varMap) (freshId + 1)
 Proof
   rpt strip_tac \\ fs[ids_unique_def]
   \\ rpt conj_tac \\ rpt strip_tac \\ fs[] \\ res_tac
   \\ fs[lookupCMLVar_appendCMLVar, lookupFloVerVar_appendCMLVar]
-  \\ every_case_tac \\ fs[lookupFloVerVar_def, lookupCMLVar_def, updateTheory.FIND_def]
+  \\ every_case_tac \\ fs[lookupFloVerVar_def, lookupCMLVar_def, appendCMLVar_def, updateTheory.FIND_def]
   \\ every_case_tac \\ rveq \\ fs[] \\ res_tac \\ fs[]
+  \\ res_tac \\ fs[]
+  \\ irule lookupCMLVar_not_mem \\ fs[lookupCMLVar_def]
 QED
 
 Theorem toFloVerExp_ids_unique:
-  ∀ varMap freshId f theIds freshId2 theExp.
-    toFloVerExp varMap freshId f = SOME (theIds, freshId2, theExp) ∧
-    ids_unique varMap freshId ⇒
+  ! varMap freshId f theIds freshId2 theExp.
+    toFloVerExp varMap freshId f = SOME (theIds, freshId2, theExp) /\
+    ids_unique varMap freshId ==>
     ids_unique theIds freshId2
 Proof
   ho_match_mp_tac toFloVerExp_ind
   \\ rpt strip_tac
   \\ fs[Once toFloVerExp_def, option_case_eq, pair_case_eq, list_case_eq]
   \\ rveq \\ fs[ids_unique_append]
-  \\ Cases_on ‘op’ \\ fs[list_case_eq, option_case_eq, pair_case_eq]
+  \\ Cases_on `op` \\ fs[list_case_eq, option_case_eq, pair_case_eq]
   \\ rveq \\ fs[]
-  \\ Cases_on ‘f’ \\ fs[option_case_eq, pair_case_eq]
+  \\ Cases_on `f` \\ fs[option_case_eq, pair_case_eq]
 QED
 
 Theorem toFloVerCmd_ids_unique:
-  ∀ varMap freshId f theIds freshId2 theCmd.
-    toFloVerCmd varMap freshId f = SOME (theIds, freshId2, theCmd) ⇒
-    ids_unique varMap freshId ⇒
+  ! varMap freshId f theIds freshId2 theCmd.
+    toFloVerCmd varMap freshId f = SOME (theIds, freshId2, theCmd) ==>
+    ids_unique varMap freshId ==>
     ids_unique theIds freshId2
 Proof
   ho_match_mp_tac toFloVerCmd_ind
@@ -370,49 +449,49 @@ Proof
 QED
 
 Theorem toFloVerExp_lookup_mono:
-  ∀ ids freshId e ids2 freshId2 fexp.
-  toFloVerExp ids freshId e = SOME (ids2, freshId2, fexp) ⇒
-  ids_unique ids freshId ⇒
-  (∀ n x. lookupFloVerVar n ids = SOME (x, n) ⇒
-   lookupFloVerVar n ids2 = SOME (x,n)) ∧
-  (∀ x n. lookupCMLVar x ids = SOME (x,n) ⇒
+  ! ids freshId e ids2 freshId2 fexp.
+  toFloVerExp ids freshId e = SOME (ids2, freshId2, fexp) ==>
+  ids_unique ids freshId ==>
+  (! n x. lookupFloVerVar n ids = SOME (x, n) ==>
+   lookupFloVerVar n ids2 = SOME (x,n)) /\
+  (! x n. lookupCMLVar x ids = SOME (x,n) ==>
    lookupCMLVar x ids2 = SOME (x,n))
 Proof
   ho_match_mp_tac toFloVerExp_ind
   \\ rpt strip_tac
-  \\ ((rename1 ‘App op exps’ \\ imp_res_tac toFloVerExp_App_cases)
+  \\ ((rename1 `App op exps` \\ imp_res_tac toFloVerExp_App_cases)
      ORELSE
-     (qpat_x_assum ‘toFloVerExp _ _ _ = SOME _’ mp_tac
+     (qpat_x_assum `toFloVerExp _ _ _ = SOME _` mp_tac
       \\ simp[Once toFloVerExp_def] \\ rpt strip_tac))
   >- (
     fs[option_case_eq, pair_case_eq] \\ rveq
     \\ fs[lookupFloVerVar_appendCMLVar, lookupFloVerVar_def, ids_unique_def, updateTheory.FIND_def]
-    \\ TOP_CASE_TAC \\ fs[] \\ rveq \\ first_x_assum (qspec_then ‘freshId’ assume_tac) \\ fs[])
+    \\ TOP_CASE_TAC \\ fs[] \\ rveq \\ first_x_assum (qspec_then `freshId` assume_tac) \\ fs[])
   >- (
     fs[option_case_eq, pair_case_eq] \\ rveq
     \\ fs[lookupCMLVar_appendCMLVar, lookupCMLVar_def, ids_unique_def, updateTheory.FIND_def]
-    \\ TOP_CASE_TAC \\ fs[] \\ rveq \\ first_x_assum (qspec_then ‘freshId’ assume_tac) \\ fs[])
+    \\ TOP_CASE_TAC \\ fs[] \\ rveq \\ first_x_assum (qspec_then `freshId` assume_tac) \\ fs[])
   >- (
      rveq \\ fs[])
   >- (
      rveq \\ fs[])
-  \\ rveq \\ fs[] \\ rpt strip_tac \\ TRY (Cases_on ‘f’) \\ fs[option_case_eq, pair_case_eq]
+  \\ rveq \\ fs[] \\ rpt strip_tac \\ TRY (Cases_on `f`) \\ fs[option_case_eq, pair_case_eq]
   \\ rveq \\ imp_res_tac toFloVerExp_ids_unique
   \\ res_tac \\ res_tac
 QED
 
 Theorem toFloVerCmd_lookup_mono:
-  ∀ ids freshId e ids2 freshId2 theCmd.
-  toFloVerCmd ids freshId e = SOME (ids2, freshId2, theCmd) ⇒
-  ids_unique ids freshId ⇒
-  (∀ n x. lookupFloVerVar n ids = SOME (x, n) ⇒
-   lookupFloVerVar n ids2 = SOME (x,n)) ∧
-  (∀ x n. lookupCMLVar x ids = SOME (x,n) ⇒
+  ! ids freshId e ids2 freshId2 theCmd.
+  toFloVerCmd ids freshId e = SOME (ids2, freshId2, theCmd) ==>
+  ids_unique ids freshId ==>
+  (! n x. lookupFloVerVar n ids = SOME (x, n) ==>
+   lookupFloVerVar n ids2 = SOME (x,n)) /\
+  (! x n. lookupCMLVar x ids = SOME (x,n) ==>
    lookupCMLVar x ids2 = SOME (x,n))
 Proof
   ho_match_mp_tac toFloVerCmd_ind
   \\ rpt strip_tac
-  \\ qpat_x_assum ‘toFloVerCmd _ _ _ = SOME _’ mp_tac
+  \\ qpat_x_assum `toFloVerCmd _ _ _ = SOME _` mp_tac
   \\ simp[Once toFloVerCmd_def] \\ rpt strip_tac
   \\ TRY (fs[option_case_eq, pair_case_eq] \\ rveq \\ imp_res_tac toFloVerExp_lookup_mono)
   \\ fs[]
@@ -428,18 +507,18 @@ Proof
 QED
 
 Theorem toFloVerExp_freevars_agree:
-  ∀ varMap freshId f theIds freshId2 theExp v.
-    toFloVerExp varMap freshId f = SOME (theIds, freshId2, theExp) ∧
-    ids_unique varMap freshId ∧
-    v ∈ domain (usedVars theExp) ⇒
-    ∃ x. lookupFloVerVar v theIds = SOME (x, v) ∧
+  ! varMap freshId f theIds freshId2 theExp v.
+    toFloVerExp varMap freshId f = SOME (theIds, freshId2, theExp) /\
+    ids_unique varMap freshId /\
+    v IN domain (usedVars theExp) ==>
+    ? x. lookupFloVerVar v theIds = SOME (x, v) /\
       x IN freevars [f]
 Proof
   ho_match_mp_tac toFloVerExp_ind
   \\ rpt strip_tac
-  \\ ((rename1 ‘App op exps’ \\ imp_res_tac toFloVerExp_App_cases)
+  \\ ((rename1 `App op exps` \\ imp_res_tac toFloVerExp_App_cases)
      ORELSE
-     (qpat_x_assum ‘toFloVerExp _ _ _ = SOME _’ mp_tac
+     (qpat_x_assum `toFloVerExp _ _ _ = SOME _` mp_tac
       \\ simp[Once toFloVerExp_def] \\ rpt strip_tac))
   \\ fs[Once toFloVerExp_def, option_case_eq, pair_case_eq, list_case_eq]
   \\ rveq
@@ -452,7 +531,7 @@ Proof
     \\ res_tac \\ fs[])
   >- (
     fs[usedVars_def])
-  \\ rveq \\ qpat_x_assum ‘_ IN domain (usedVars _)’ mp_tac
+  \\ rveq \\ qpat_x_assum `_ IN domain (usedVars _)` mp_tac
   \\ simp[Once usedVars_def, domain_union] \\ rpt strip_tac
   \\ imp_res_tac toFloVerExp_ids_unique
   \\ TRY (fs[] \\ res_tac \\ fsrw_tac [SATISFY_ss] [freevars_def])
@@ -461,11 +540,11 @@ Proof
 QED
 
 Theorem toFloVerCmd_freevars_agree:
-  ∀ varMap freshId f theIds freshId2 theCmd v.
-    toFloVerCmd varMap freshId f = SOME (theIds, freshId2, theCmd) ∧
-    ids_unique varMap freshId ∧
-    v ∈ domain (freeVars theCmd) ⇒
-    ∃ x. lookupFloVerVar v theIds = SOME (x, v) ∧
+  ! varMap freshId f theIds freshId2 theCmd v.
+    toFloVerCmd varMap freshId f = SOME (theIds, freshId2, theCmd) /\
+    ids_unique varMap freshId /\
+    v IN domain (freeVars theCmd) ==>
+    ? x. lookupFloVerVar v theIds = SOME (x, v) /\
       x IN freevars [f]
 Proof
   ho_match_mp_tac toFloVerCmd_ind
@@ -475,28 +554,28 @@ Proof
   \\ fs[]
   \\ imp_res_tac toFloVerExp_ids_unique
   \\ imp_res_tac toFloVerCmd_ids_unique
-  \\ qpat_x_assum ‘v IN domain (freeVars _)’ mp_tac
-  \\ rename1 ‘ids_unique (appendCMLVar (Short x) freshId3 ids2) (freshId3 + 1)’
-  \\ ‘ids_unique (appendCMLVar (Short x) freshId3 ids2) (freshId3 + 1)’
+  \\ qpat_x_assum `v IN domain (freeVars _)` mp_tac
+  \\ rename1 `ids_unique (appendCMLVar (Short x) freshId3 ids2) (freshId3 + 1)`
+  \\ `ids_unique (appendCMLVar (Short x) freshId3 ids2) (freshId3 + 1)`
      by (irule ids_unique_append \\ fs[])
   \\ fs[]
   \\ simp[Once freeVars_def, domain_union] \\ rpt strip_tac \\ fs[]
   >- (
     imp_res_tac toFloVerExp_freevars_agree \\ fs[] \\ rveq
     \\ imp_res_tac toFloVerCmd_lookup_mono \\ fs[]
-    \\ rename1 ‘lookupFloVerVar n ids2 = SOME (y,n)’
-    \\ ‘lookupFloVerVar n (appendCMLVar (Short x) freshId3 ids2) = SOME (y,n)’
+    \\ rename1 `lookupFloVerVar n ids2 = SOME (y,n)`
+    \\ `lookupFloVerVar n (appendCMLVar (Short x) freshId3 ids2) = SOME (y,n)`
       by (fs[lookupFloVerVar_appendCMLVar, lookupFloVerVar_def,
              updateTheory.FIND_def])
     \\ res_tac \\ fs[freevars_def])
   \\ first_x_assum drule \\ fs[freevars_def] \\ disch_then assume_tac
   \\ fs[]
-  \\ Cases_on ‘x' = Short x’ \\ fs[]
+  \\ Cases_on `x' = Short x` \\ fs[]
   \\ rveq
-  \\ ‘lookupCMLVar (Short x) ids3 = SOME (Short x, v)’
+  \\ `lookupCMLVar (Short x) ids3 = SOME (Short x, v)`
     by (fs[ids_unique_def])
   \\ fs[appendCMLVar_def]
-  \\ ‘lookupCMLVar (Short x) ((Short x, freshId3)::ids2) = SOME (Short x, freshId3)’
+  \\ `lookupCMLVar (Short x) ((Short x, freshId3)::ids2) = SOME (Short x, freshId3)`
      by EVAL_TAC
   \\ rfs[]
   \\ imp_res_tac toFloVerCmd_lookup_mono
@@ -504,21 +583,21 @@ Proof
 QED
 
 Theorem toRExp_usedVars_agree:
-  ∀ v e.
-    v IN (domain (usedVars (toRExp e))) ⇒
+  ! v e.
+    v IN (domain (usedVars (toRExp e))) ==>
     v IN domain (usedVars e)
 Proof
-  Induct_on ‘e’ \\ simp[Once usedVars_def, toRExp_def, domain_union]
+  Induct_on `e` \\ simp[Once usedVars_def, toRExp_def, domain_union]
   \\ rpt strip_tac \\ res_tac
   \\ simp[Once usedVars_def, domain_union]
 QED
 
 Theorem toRCmd_freeVars_agree:
-  ∀ v theCmd.
-  v IN (domain (freeVars (toRCmd theCmd))) ⇒
+  ! v theCmd.
+  v IN (domain (freeVars (toRCmd theCmd))) ==>
   v IN domain (freeVars theCmd)
 Proof
-  Induct_on ‘theCmd’ \\ simp[Once freeVars_def, toRCmd_def, domain_union]
+  Induct_on `theCmd` \\ simp[Once freeVars_def, toRCmd_def, domain_union]
   \\ rpt strip_tac
   \\ imp_res_tac toRExp_usedVars_agree
   \\ res_tac
